Soundness.thy
@@ -2,20 +2,61 @@ theory Soundness
   imports Semantics
 begin
 
-lemma triple_rule_parallel:
+
+lemma htriple_ndet:
   fixes a b :: \<open>('x,'p) action process\<close>
   assumes
-    \<open>\<lbrace> pa \<rbrace> interp_act a \<lbrace> qa \<rbrace>\<close>
-    \<open>\<lbrace> pb \<rbrace> interp_act b \<lbrace> qb \<rbrace>\<close>
-  shows \<open>\<lbrace> pa \<^emph> pb \<rbrace> interp_act (a \<parallel> b) \<lbrace> qa \<^emph> qb \<rbrace>\<close>
-  using assms
+    \<open>\<lbrace> p1 \<rbrace> a \<lbrace> q1 \<rbrace>\<close>
+    \<open>\<lbrace> p2 \<rbrace> b \<lbrace> q2 \<rbrace>\<close>
+  shows 
+    \<open>\<lbrace> p1 \<sqinter> p2 \<rbrace>  (a + b) \<lbrace> q1 \<squnion> q2 \<rbrace>\<close>
   sorry
+
+
+lemma htriple_seq:
+  fixes a b :: \<open>('x,'p) action process\<close>
+  assumes
+    \<open>\<lbrace> p \<rbrace> a \<lbrace> q \<rbrace>\<close>
+    \<open>\<lbrace> q \<rbrace> b \<lbrace> r \<rbrace>\<close>
+  shows \<open>\<lbrace> p \<rbrace>  (a \<triangleright> b) \<lbrace> r \<rbrace>\<close>
+  using assms htriple'_def seq_process_def  leD less_eq_process_def
+      zero_process_def 
+  sorry
+
+lemma htriple_parallel:
+  fixes a b :: \<open>('x,'p) action process\<close>
+  assumes
+    \<open>\<lbrace> p1 \<rbrace>  a \<lbrace> q1 \<rbrace>\<close>
+    \<open>\<lbrace> p2 \<rbrace>  b \<lbrace> q2 \<rbrace>\<close>
+  shows 
+    \<open>\<lbrace> p1 \<^emph> p2 \<rbrace>  (a * b) \<lbrace> q1 \<^emph> q2 \<rbrace>\<close>
+  sorry
+
+
+lemma htriple_zero: \<open>\<lbrace> \<bottom> \<rbrace> 0 \<lbrace> q \<rbrace>\<close>  sorry
+
+lemma htriple_one: \<open>\<lbrace> p \<rbrace> 1 \<lbrace> p \<rbrace>\<close> 
+  using htriple'_def htriple_def one_process.rep_eq sorry
+
+
+(*
+
+lemma 
+ fixes c1 c2 :: \<open>('x,'p) action process\<close>
+  assumes
+    \<open>\<lbrace> pa \<rbrace> \<lambda>s s'. \<forall>t1\<in>proctr c1. s \<sim>t1\<leadsto>\<^sup>* s' \<lbrace> qa \<rbrace>\<close>
+    \<open> \<lbrace> pb \<rbrace> \<lambda>s s'. \<forall>t2\<in>proctr c2. s \<sim>t2\<leadsto>\<^sup>* s' \<lbrace> qb \<rbrace>\<close>
+  shows \<open>\<lbrace> pa \<^emph> pb \<rbrace> \<lambda>s s'. \<forall>t1_t2\<in>proctr (c1 * c2). s \<sim>t1_t2\<leadsto>\<^sup>* s' \<lbrace> qa \<^emph> qb \<rbrace>\<close>
+  oops
+*)
 
 lemma triple_rule_frame:
   fixes a b :: \<open>('x,'p) action process\<close>
-  assumes \<open>\<lbrace> p \<rbrace> interp_act a \<lbrace> q \<rbrace>\<close>
-  shows \<open>\<lbrace> p \<^emph> r \<rbrace> interp_act a \<lbrace> q \<^emph> r \<rbrace>\<close>
+  assumes \<open>\<lbrace> p \<rbrace>  a \<lbrace> q \<rbrace>\<close>
+  shows \<open>\<lbrace> p \<^emph> r \<rbrace> a \<lbrace> q \<^emph> r \<rbrace>\<close>
   using assms
   sorry
+
+
 
 end
